module bool-thms2 where

open import bool
open import eq
open import product
open import sum

ff-imp : âˆ€ (b : ğ”¹) â†’ ff imp b â‰¡ tt
ff-imp ff = refl
ff-imp tt = refl

imp-tt : âˆ€ (b : ğ”¹) â†’ b imp tt â‰¡ tt
imp-tt ff = refl
imp-tt tt = refl

imp-ff : âˆ€ (b : ğ”¹) â†’ b imp ff â‰¡ ~ b
imp-ff tt = refl
imp-ff ff = refl

tt-imp : âˆ€ (b : ğ”¹) â†’ tt imp b â‰¡ b
tt-imp tt = refl
tt-imp ff = refl

&&-tt : âˆ€ (b : ğ”¹) â†’ b && tt â‰¡ b
&&-tt tt = refl
&&-tt ff = refl

||-ff : âˆ€ (b : ğ”¹) â†’ b || ff â‰¡ b
||-ff tt = refl
||-ff ff = refl

&&-contra : âˆ€ (b : ğ”¹) â†’ b && ~ b â‰¡ ff
&&-contra ff = refl
&&-contra tt = refl

&&-comm : âˆ€ (b1 b2 : ğ”¹) â†’ b1 && b2 â‰¡ b2 && b1
&&-comm ff ff = refl
&&-comm ff tt = refl
&&-comm tt ff = refl
&&-comm tt tt = refl

||-comm : âˆ€ (b1 b2 : ğ”¹) â†’ b1 || b2 â‰¡ b2 || b1
||-comm ff ff = refl
||-comm ff tt = refl
||-comm tt ff = refl
||-comm tt tt = refl

&&-assoc : âˆ€ (b1 b2 b3 : ğ”¹) â†’ b1 && (b2 && b3) â‰¡ (b1 && b2) && b3
&&-assoc ff _ _ = refl
&&-assoc tt _ _ = refl

||-assoc : âˆ€ (b1 b2 b3 : ğ”¹) â†’ b1 || (b2 || b3) â‰¡ (b1 || b2) || b3
||-assoc tt _ _ = refl
||-assoc ff _ _ = refl

~-over-&& : âˆ€ (b1 b2 : ğ”¹) â†’ ~ ( b1 && b2 ) â‰¡ (~ b1 || ~ b2)
~-over-&& tt _ = refl
~-over-&& ff _ = refl

~-over-|| : âˆ€ (b1 b2 : ğ”¹) â†’ ~ ( b1 || b2 ) â‰¡ (~ b1 && ~ b2)
~-over-|| tt _ = refl
~-over-|| ff _ = refl

&&-over-||-l : âˆ€ (a b c : ğ”¹) â†’ a && (b || c) â‰¡ (a && b) || (a && c)
&&-over-||-l tt _ _ = refl
&&-over-||-l ff _ _ = refl 

&&-over-||-r : âˆ€ (a b c : ğ”¹) â†’ (a || b) && c â‰¡ (a && c) || (b && c)
&&-over-||-r tt tt tt = refl
&&-over-||-r tt tt ff = refl
&&-over-||-r tt ff tt = refl
&&-over-||-r tt ff ff = refl
&&-over-||-r ff tt tt = refl
&&-over-||-r ff tt ff = refl
&&-over-||-r ff ff tt = refl
&&-over-||-r ff ff ff = refl

||-over-&&-l : âˆ€ (a b c : ğ”¹) â†’ a || (b && c) â‰¡ (a || b) && (a || c)
||-over-&&-l tt _ _ = refl
||-over-&&-l ff _ _ = refl 

||-over-&&-r : âˆ€ (a b c : ğ”¹) â†’ (a && b) || c â‰¡ (a || c) && (b || c)
||-over-&&-r tt _ _ = refl
||-over-&&-r ff _ ff = refl
||-over-&&-r ff tt tt = refl
||-over-&&-r ff ff tt = refl

&&-congâ‚ : âˆ€ {b1 b1' b2 : ğ”¹} â†’ b1 â‰¡ b1' â†’ b1 && b2 â‰¡ b1' && b2
&&-congâ‚ refl = refl

&&-congâ‚‚ : âˆ€ {b1 b2 b2' : ğ”¹} â†’ b2 â‰¡ b2' â†’ b1 && b2 â‰¡ b1 && b2'
&&-congâ‚‚ refl = refl 

&&-intro : âˆ€ {b1 b2 : ğ”¹} â†’ b1 â‰¡ tt â†’ b2 â‰¡ tt â†’ b1 && b2 â‰¡ tt
&&-intro{tt}{tt} _ _ = refl
&&-intro{tt}{ff} _ ()
&&-intro{ff}{tt} () _
&&-intro{ff}{ff} () _

||-intro1 : âˆ€ {b1 b2 : ğ”¹} â†’ b1 â‰¡ tt â†’ b1 || b2 â‰¡ tt
||-intro1 {tt} p = refl
||-intro1 {ff} ()

&&-elim : âˆ€ {b1 b2 : ğ”¹} â†’ b1 && b2 â‰¡ tt â†’ b1 â‰¡ tt âˆ§ b2 â‰¡ tt 
&&-elim{tt}{tt} _ = refl , refl
&&-elim{ff}{_} ()
&&-elim{tt}{ff} ()

&&-elim1 : âˆ€ {b1 b2 : ğ”¹} â†’ b1 && b2 â‰¡ tt â†’ b1 â‰¡ tt
&&-elim1 p with &&-elim p
&&-elim1 _ | p , _ = p

&&-elim2 : âˆ€ {b1 b2 : ğ”¹} â†’ b1 && b2 â‰¡ tt â†’ b2 â‰¡ tt
&&-elim2{b1} p with &&-elim{b1} p
&&-elim2 _ | _ , p = p

||-elim : âˆ€ {b1 b2 : ğ”¹} â†’ b1 || b2 â‰¡ tt â†’ b1 â‰¡ tt âˆ¨ b2 â‰¡ tt
||-elim {tt} refl = injâ‚ refl
||-elim {ff} refl = injâ‚‚ refl

~-cong : âˆ€ {b b' : ğ”¹} â†’ b â‰¡ b' â†’ ~ b â‰¡ ~ b'
~-cong refl = refl

ite-congâ‚ : âˆ€{â„“}{A : Set â„“} {b b' : ğ”¹}(x y : A) â†’ b â‰¡ b' â†’ (if b then x else y) â‰¡ (if b' then x else y)
ite-congâ‚ x y refl = refl

ite-congâ‚‚ : âˆ€{â„“}{A : Set â„“} (b : ğ”¹){x x' : A}(y : A) â†’ x â‰¡ x' â†’ (if b then x else y) â‰¡ (if b then x' else y)
ite-congâ‚‚ b y refl = refl

ite-congâ‚ƒ : âˆ€{â„“}{A : Set â„“} (b : ğ”¹)(x : A){y y' : A} â†’ y â‰¡ y' â†’ (if b then x else y) â‰¡ (if b then x else y')
ite-congâ‚ƒ b x refl = refl

&&-split : âˆ€ {b b' : ğ”¹} â†’ b || b' â‰¡ ff â†’ b â‰¡ ff âŠ b' â‰¡ ff
&&-split {tt} ()
&&-split {ff}{tt} ()
&&-split {ff}{ff} p = injâ‚ refl

-----------------------------------
-- Theorems about imp
-----------------------------------
imp-same : âˆ€ (b : ğ”¹) â†’ b imp b â‰¡ tt
imp-same ff = refl
imp-same tt = refl

imp-to-|| : âˆ€ (b1 b2 : ğ”¹) â†’ (b1 imp b2) â‰¡ (~ b1 || b2)
imp-to-|| ff _ = refl
imp-to-|| tt _ = refl

imp-mp : âˆ€ {b b' : ğ”¹} â†’ b imp b' â‰¡ tt â†’ b â‰¡ tt â†’ b' â‰¡ tt 
imp-mp {tt} {tt} p refl = refl
imp-mp {ff} {ff} p q = q
imp-mp {tt} {ff} p q = p
imp-mp {ff} {tt} p q = refl

imp-antisymm : âˆ€ {b1 b2 : ğ”¹} â†’ b1 imp b2 â‰¡ tt â†’ b2 imp b1 â‰¡ tt â†’ b1 â‰¡ b2
imp-antisymm{tt}{tt} p q = refl
imp-antisymm{tt}{ff} () q 
imp-antisymm{ff}{tt} p ()
imp-antisymm{ff}{ff} p q = refl

-----------------------------------
-- Theorems about xor
-----------------------------------
ff-xor : âˆ€ (b : ğ”¹) â†’ ff xor b â‰¡ b
ff-xor tt = refl
ff-xor ff = refl

tt-xor : âˆ€ (b : ğ”¹) â†’ tt xor b â‰¡ ~ b
tt-xor tt = refl
tt-xor ff = refl

~-xor-distrb : âˆ€ (a b : ğ”¹) â†’ ~ (a xor b) â‰¡ ~ a xor b
~-xor-distrb tt tt = refl
~-xor-distrb tt ff = refl
~-xor-distrb ff tt = refl
~-xor-distrb ff ff = refl

xor-distrib-&& : âˆ€ (x y : ğ”¹) â†’ x xor (y && x) â‰¡ ~ y && x
xor-distrib-&& tt tt = refl
xor-distrib-&& tt ff = refl
xor-distrib-&& ff tt = refl
xor-distrib-&& ff ff = refl

xor~hop : âˆ€ (a b : ğ”¹) â†’ ~ a xor b â‰¡ a xor ~ b
xor~hop tt tt = refl
xor~hop tt ff = refl
xor~hop ff tt = refl
xor~hop ff ff = refl

xor-comm : âˆ€ (b1 b2 : ğ”¹) â†’ b1 xor b2 â‰¡ b2 xor b1
xor-comm tt tt = refl
xor-comm tt ff = refl
xor-comm ff tt = refl
xor-comm ff ff = refl

xor-assoc : (b1 b2 b3 : ğ”¹) â†’ b1 xor (b2 xor b3) â‰¡ (b1 xor b2) xor b3
xor-assoc tt tt tt = refl
xor-assoc tt tt ff = refl
xor-assoc tt ff tt = refl
xor-assoc tt ff ff = refl
xor-assoc ff tt tt = refl
xor-assoc ff tt ff = refl
xor-assoc ff ff tt = refl
xor-assoc ff ff ff = refl

xor-anti-idem : (b : ğ”¹) â†’ b xor b â‰¡ ff
xor-anti-idem tt = refl
xor-anti-idem ff = refl

xor-â‰¡ : {b1 b2 : ğ”¹} â†’ b1 xor b2 â‰¡ ff â†’ b1 â‰¡ b2
xor-â‰¡ {tt} {tt} p = refl
xor-â‰¡ {tt} {ff} ()
xor-â‰¡ {ff} {tt} ()
xor-â‰¡ {ff} {ff} p = refl

-----------------------------------
-- Theorems about nor, nand
-----------------------------------

nor-not : âˆ€ (b : ğ”¹) â†’ b nor b â‰¡ ~ b
nor-not tt = refl
nor-not ff = refl

nor-or : âˆ€ (b1 b2 : ğ”¹) â†’ (b1 nor b2) nor (b1 nor b2) â‰¡ b1 || b2
nor-or tt b2 = refl
nor-or ff tt = refl
nor-or ff ff = refl

nor-and : âˆ€ (b1 b2 : ğ”¹) â†’ (b1 nor b1) nor (b2 nor b2) â‰¡ b1 && b2
nor-and tt tt = refl
nor-and tt ff = refl
nor-and ff b2 = refl

nor-comm : âˆ€ (b1 b2 : ğ”¹) â†’ b1 nor b2 â‰¡ b2 nor b1
nor-comm tt tt = refl
nor-comm tt ff = refl
nor-comm ff tt = refl
nor-comm ff ff = refl

nand-comm : âˆ€ (b1 b2 : ğ”¹) â†’ b1 nand b2 â‰¡ b2 nand b1
nand-comm tt tt = refl
nand-comm tt ff = refl
nand-comm ff tt = refl
nand-comm ff ff = refl

