open import lib
open import sum

module grammar (form : Set)(_eq_ : form â†’ form â†’ ğ”¹)(drop-form : (x y : form) â†’ x â‰¡ y â†’ x eq y â‰¡ tt)(rise-form : (x y : form) â†’ x eq y â‰¡ tt â†’ x â‰¡ y) where

infix 7 _â‡’_

data production : Set where
  _â‡’_ : form â†’ ğ•ƒ (form âŠ char) â†’ production

record grammar {numprods : â„•} : Set where
  constructor  _,_
  field
    start : form
    prods : ğ• production numprods

open grammar

splice : â„• â†’ ğ•ƒ (form âŠ char) â†’ form â†’ ğ•ƒ (form âŠ char) â†’ ğ•ƒ (form âŠ char)
splice x [] _ _ = []
splice 0 ((injâ‚ s) :: ss) s' ss' with s eq s'
... | tt = ss' ++ ss
... | ff = (injâ‚ s) :: ss
splice 0 (x :: ss) s' ss' = x :: ss
splice (suc n) (s :: ss) s' ss' = s :: splice n ss s' ss'

ğ•ƒinjâ‚‚ : âˆ€{â„“ â„“'}{B : Set â„“}{A : Set â„“'} â†’ ğ•ƒ A â†’ ğ•ƒ (B âŠ A)
ğ•ƒinjâ‚‚ (x :: xs) = (injâ‚‚ x) :: ğ•ƒinjâ‚‚ xs
ğ•ƒinjâ‚‚ [] = []

ğ•ƒinjâ‚ : âˆ€{â„“ â„“'}{B : Set â„“}{A : Set â„“'} â†’ ğ•ƒ A â†’ ğ•ƒ (A âŠ B)
ğ•ƒinjâ‚ (x :: xs) = (injâ‚ x) :: ğ•ƒinjâ‚ xs
ğ•ƒinjâ‚ [] = []

data derivation{numprods : â„•} {g : grammar{numprods}} : ğ•ƒ (form âŠ char) â†’ ğ•ƒ char â†’ Set where
  end : {ss : ğ•ƒ char} â†’ derivation (ğ•ƒinjâ‚‚ ss) ss
  step : âˆ€ {ss1 ss1' : ğ•ƒ (form âŠ char)}{ss2 : ğ•ƒ char}{s : form}{ss : ğ•ƒ (form âŠ char)} â†’ 
           (m n : â„•) â†’ (p : n < numprods â‰¡ tt) â†’ 
           nthğ• n p (prods g) â‰¡ (s â‡’ ss) â†’ 
           m < length ss1 â‰¡ tt â†’
           splice m ss1 s ss â‰¡ ss1' â†’ 
           derivation {g = g} ss1' ss2 â†’
           derivation ss1 ss2

splice-concat : âˆ€{l1 l2 target final : ğ•ƒ (form âŠ char)}{n : â„•}{slice : form} â†’ splice n l1 slice target â‰¡ final â†’ splice (n + (length l2)) (l2 ++ l1) slice target â‰¡ l2 ++ final
splice-concat{l2 = []}{n = n} pr rewrite +0 n = pr
splice-concat{l1}{x :: xs}{n = n} pr rewrite +suc n (length xs) | splice-concat{l1}{l2 = xs} pr = refl

_=formâŠchar_ : (x y : form âŠ char) â†’ ğ”¹
_=formâŠchar_ = =âŠ _eq_ _=char_

formâŠchar-drop : (x y : form âŠ char) â†’ x â‰¡ y â†’ x =formâŠchar y â‰¡ tt 
formâŠchar-drop = â‰¡âŠ-to-= _eq_ _=char_ drop-form â‰¡char-to-=

formâŠchar-rise : (x y : form âŠ char) â†’ x =formâŠchar y â‰¡ tt â†’ x â‰¡ y
formâŠchar-rise = =âŠ-to-â‰¡ _eq_ _=char_ rise-form =char-to-â‰¡


splice-concat2 : âˆ€{l1 l2 target final : ğ•ƒ (form âŠ char)}{n : â„•}{slice : form} â†’ splice n l1 slice target â‰¡ final â†’ n < length l1 â‰¡ tt â†’ splice n (l1 ++ l2) slice target â‰¡ final ++ l2
splice-concat2{[]}{n = n} pr1 pr2 rewrite <-0 n = ğ”¹-contra pr2
splice-concat2{injâ‚ x :: xs}{l2}{target}{n = 0}{slice} pr1 pr2 with x eq slice
...| tt rewrite (sym pr1) | ++[] target | ++-assoc target xs l2 = refl
...| ff rewrite (sym pr1) = refl
splice-concat2{injâ‚‚ x :: xs}{l2}{target}{n = 0}{slice} pr1 pr2 rewrite (sym pr1) = refl
splice-concat2{x :: xs}{l2}{target}{[]}{suc n} pr1 pr2 with pr1 
...| ()
splice-concat2{x :: xs}{l2}{target}{f :: fs}{suc n}{slice} pr1 pr2 with =ğ•ƒ-from-â‰¡ _=formâŠchar_ formâŠchar-drop pr1 
...| s1 rewrite splice-concat2{xs}{l2}{target}{fs}{n}{slice} (â‰¡ğ•ƒ-from-={l1 = splice n xs slice target}{fs} _=formâŠchar_ formâŠchar-rise (&&-snd{x =formâŠchar f} s1)) pr2 | formâŠchar-rise x f (&&-fst{x =formâŠchar f} s1) = refl 

length+ : âˆ€{â„“}{A : Set â„“}(l1 l2 : ğ•ƒ A) â†’ length (l1 ++ l2) â‰¡ length l1 + length l2
length+ [] l2 = refl
length+ (x :: xs) l2 rewrite length+ xs l2 = refl

<-h1 : âˆ€{x y a : â„•} â†’ x < y â‰¡ tt â†’ x + a < y + a â‰¡ tt
<-h1{x}{y}{0} p rewrite +0 x | +0 y = p
<-h1{x}{y}{suc n} p rewrite +suc y n | +suc x n = <-h1{x}{y}{n} p

<-h2 : âˆ€{a x y : â„•} â†’ a < x â‰¡ tt â†’ a < x + y â‰¡ tt
<-h2{a}{x}{0} p rewrite +0 x = p
<-h2{a}{x}{suc y} p rewrite +suc x y with <-h2{a}{x}{y} p | <-suc (x + y)
...| pr1 | pr2 = <-trans{a}{x + y}{suc (x + y)} pr1 pr2

lengthğ•ƒinjâ‚‚ : âˆ€{â„“ â„“'}{A : Set â„“}{B : Set â„“'} â†’ (l : ğ•ƒ A) â†’ length (ğ•ƒinjâ‚‚{B = B} l) â‰¡ length l
lengthğ•ƒinjâ‚‚{B = B} (x :: xs) rewrite lengthğ•ƒinjâ‚‚{B = B} xs = refl
lengthğ•ƒinjâ‚‚ [] = refl

ğ•ƒinjâ‚‚++ : âˆ€{â„“ â„“'}{A : Set â„“}{B : Set â„“'} â†’ (l1 l2 : ğ•ƒ A) â†’ ğ•ƒinjâ‚‚{B = B} (l1 ++ l2) â‰¡ ğ•ƒinjâ‚‚ l1 ++ ğ•ƒinjâ‚‚ l2
ğ•ƒinjâ‚‚++ [] l2 = refl
ğ•ƒinjâ‚‚++{B = B} (x :: xs) l2 rewrite ğ•ƒinjâ‚‚++{B = B} xs l2 = refl

infixr 10 _deriv++_

_deriv++_ : {l2 l4 : ğ•ƒ char}{l1 l3 : ğ•ƒ (form âŠ char)}{n : â„•}{gr : grammar{n}} â†’ derivation{g = gr} l1 l2 â†’ derivation{g = gr} l3 l4 â†’ derivation{g = gr} (l1 ++ l3) (l2 ++ l4)
_deriv++_{l2}{l4} end end rewrite sym (ğ•ƒinjâ‚‚++{B = form} l2 l4) = end
_deriv++_{l2}{l4}{l1}{l3} f (step{ss1' = ss1'}{s = s}{ss} a b pr1 pr2 pr3 pr4 next) with <-h1{a}{length l3}{length l1} pr3
...| pr5 rewrite +comm (length l3) (length l1) | (sym (length+ l1 l3)) =  step{ss1 = l1 ++ l3}{l1 ++ ss1'}{l2 ++ l4} (a + (length l1)) b pr1 pr2 pr5 (splice-concat{l3}{l1} pr4) (_deriv++_ f next) 
_deriv++_{l2}{l4}{l1} (step{ss1' = ss1'}{s = s}{ss} a b pr1 pr2 pr3 pr4 next) end with <-h2{a}{length l1}{length (ğ•ƒinjâ‚‚{B = form} l4)} pr3
...| pr5 rewrite sym (length+ l1 (ğ•ƒinjâ‚‚ l4)) = step{ss1 = l1 ++ ğ•ƒinjâ‚‚ l4}{ss1' ++ ğ•ƒinjâ‚‚ l4}{l2 ++ l4} a b pr1 pr2 pr5 (splice-concat2{l1}{ğ•ƒinjâ‚‚ l4} pr4 pr3) (_deriv++_ next end)

