module list-thms where

-- see list-thms2 for more 

open import bool
open import bool-thms
open import functions
open import list
open import nat
open import nat-thms
open import product-thms
open import logic

++[] : âˆ€{â„“}{A : Set â„“} â†’ (l : ğ•ƒ A) â†’ l ++ [] â‰¡ l
++[] [] = refl
++[] (x :: xs) rewrite ++[] xs = refl

++-assoc : âˆ€ {â„“}{A : Set â„“} (l1 l2 l3 : ğ•ƒ A) â†’ 
           (l1 ++ l2) ++ l3 â‰¡ l1 ++ (l2 ++ l3)
++-assoc [] l2 l3 = refl
++-assoc (x :: xs) l2 l3 rewrite ++-assoc xs l2 l3 = refl

length-++ : âˆ€{â„“}{A : Set â„“}(l1 l2 : ğ•ƒ A) â†’ 
            length (l1 ++ l2) â‰¡ (length l1) + (length l2)
length-++ [] l2 = refl
length-++ (h :: t) l2 rewrite length-++ t l2 = refl

map-append : âˆ€ {â„“ â„“'} {A : Set â„“} {B : Set â„“'} â†’ 
             (f : A â†’ B) (l1 l2 : ğ•ƒ A) â†’ 
             map f (l1 ++ l2) â‰¡ (map f l1) ++ (map f l2)
map-append f [] l2 = refl
map-append f (x :: xs) l2 rewrite map-append f xs l2 = refl

map-compose : âˆ€ {â„“ â„“' â„“''} {A : Set â„“} {B : Set â„“'}{C : Set â„“''} â†’ 
             (f : B â†’ C) (g : A â†’ B) (l : ğ•ƒ A) â†’ 
             map f (map g l) â‰¡ map (f âˆ˜ g) l
map-compose f g [] = refl
map-compose f g (x :: xs) rewrite map-compose f g xs = refl

foldr-append : âˆ€{â„“â‚ â„“â‚‚}{A : Set â„“â‚}{B : Set â„“â‚‚}{lâ‚ lâ‚‚ : ğ•ƒ (A â†’ ğ•ƒ B)}{a : A}
  â†’ (foldr (Î» f â†’ _++_ (f a)) [] lâ‚) ++ (foldr (Î» f â†’ _++_ (f a)) [] lâ‚‚) â‰¡ foldr (Î» f â†’ _++_ (f a)) [] (lâ‚ ++ lâ‚‚)
foldr-append {lâ‚ = []}{_}{a} = refl
foldr-append {lâ‚ = x :: lâ‚}{lâ‚‚}{a}
 rewrite
    ++-assoc (x a) (foldr (Î» f â†’ _++_ (f a)) [] lâ‚) (foldr (Î» f â†’ _++_ (f a)) [] lâ‚‚)
  | foldr-append {lâ‚ = lâ‚}{lâ‚‚}{a}
 = refl
 
invertğ•ƒ : âˆ€{â„“}{A : Set â„“}{t : A}{ts : ğ•ƒ A} â†’ t :: ts â‰¢ []
invertğ•ƒ ()

length-repeat : âˆ€{â„“}{A : Set â„“} (n : â„•) (a : A) â†’ length (repeat n a) â‰¡ n
length-repeat 0 a = refl
length-repeat (suc n) a rewrite length-repeat n a = refl

map-repeat : âˆ€ {â„“ â„“'}{A : Set â„“}{B : Set â„“'}(n : â„•)(a : A)(f : A â†’ B) â†’ map f (repeat n a) â‰¡ repeat n (f a)
map-repeat 0 a f = refl
map-repeat (suc x) a f rewrite map-repeat x a f = refl

length-map : âˆ€{â„“ â„“'} {A : Set â„“} {B : Set â„“'} (f : A â†’ B)(l : ğ•ƒ A) â†’ length (map f l) â‰¡ length l
length-map f [] = refl
length-map f (head :: tail) rewrite length-map f tail = refl

length-reverse-helper : âˆ€{â„“}{A : Set â„“}(h l : ğ•ƒ A) â†’ 
                      length (reverse-helper h l) â‰¡ length h + length l
length-reverse-helper h [] rewrite +0 (length h) = refl
length-reverse-helper h (x :: xs) rewrite length-reverse-helper (x :: h) xs = sym (+suc (length h) (length xs))

length-reverse : âˆ€{â„“}{A : Set â„“}(l : ğ•ƒ A) â†’ length (reverse l) â‰¡ length l
length-reverse l = length-reverse-helper [] l

reverse-++h : âˆ€{â„“}{A : Set â„“}(l1 l2 : ğ•ƒ A) â†’ reverse-helper l1 l2 â‰¡ reverse-helper [] l2 ++ l1
reverse-++h l1 [] = refl
reverse-++h l1 (x :: xs) rewrite reverse-++h (x :: l1) xs | reverse-++h (x :: []) xs | ++-assoc (reverse xs) (x :: []) l1 = refl

reverse-++ : âˆ€{â„“}{A : Set â„“}(l1 l2 : ğ•ƒ A) â†’ reverse(l1 ++ l2) â‰¡ reverse(l2) ++ reverse(l1)
reverse-++ [] l2 rewrite ++[] (reverse l2) = refl
reverse-++ (x :: xs) l2 rewrite reverse-++h (x :: []) (xs ++ l2) | reverse-++ xs l2 | ++-assoc (reverse l2) (reverse xs) (x :: []) | sym (reverse-++h (x :: []) xs) = refl 

=ğ•ƒ-refl : âˆ€{â„“}{A : Set â„“}{l1 : ğ•ƒ A} â†’ (eq : A â†’ A â†’ ğ”¹) â†’ ((x y : A) â†’ x â‰¡ y â†’ eq x y â‰¡ tt) â†’ =ğ•ƒ eq l1 l1 â‰¡ tt
=ğ•ƒ-refl{l1 = []} eq rise = refl
=ğ•ƒ-refl{l1 = x :: xs} eq rise = &&-combo (rise x x refl) (=ğ•ƒ-refl{l1 = xs} eq rise)

â‰¡ğ•ƒ-from-= : âˆ€{â„“}{A : Set â„“}{l1 l2 : ğ•ƒ A} â†’ (eq : A â†’ A â†’ ğ”¹) â†’ ((x y : A) â†’ eq x y â‰¡ tt â†’ x â‰¡ y) â†’ =ğ•ƒ eq l1 l2 â‰¡ tt â†’ l1 â‰¡ l2
â‰¡ğ•ƒ-from-={l1 = []}{[]} eq drop p = refl
â‰¡ğ•ƒ-from-={l1 = x :: xs}{[]} eq drop ()
â‰¡ğ•ƒ-from-={l1 = []}{y :: ys} eq drop ()
â‰¡ğ•ƒ-from-={l1 = x :: xs}{y :: ys} eq drop p rewrite â‰¡ğ•ƒ-from-={l1 = xs} eq drop (&&-snd{eq x y}{=ğ•ƒ eq xs ys} p) |  drop x y (&&-fst p) = refl 

=ğ•ƒ-from-â‰¡ : âˆ€{â„“}{A : Set â„“}{l1 l2 : ğ•ƒ A} â†’ (eq : A â†’ A â†’ ğ”¹) â†’ ((x y : A) â†’ x â‰¡ y â†’ eq x y â‰¡ tt) â†’ l1 â‰¡ l2  â†’ =ğ•ƒ eq l1 l2 â‰¡ tt
=ğ•ƒ-from-â‰¡{l2 = l2} eq rise p rewrite p  = =ğ•ƒ-refl{l1 = l2} eq rise 

multi++-assoc : âˆ€{â„“}{A : Set â„“} â†’ (Ls : ğ•ƒ (ğ•ƒ A)) â†’ (l0 : ğ•ƒ A) â†’ (foldr _++_ [] Ls) ++ l0 â‰¡ (foldr _++_ [] (Ls ++ [ l0 ]))
multi++-assoc [] l' rewrite ++[] l' = refl
multi++-assoc (l :: ls) l' rewrite ++-assoc l (foldr _++_ [] ls) l' | multi++-assoc ls l' = refl

concat-foldr : âˆ€{â„“}{A : Set â„“} â†’ (ls : ğ•ƒ (ğ•ƒ A)) â†’ (l : ğ•ƒ A) â†’ concat ls ++ l â‰¡ foldr _++_ l ls
concat-foldr [] l = refl
concat-foldr (l' :: ls) l rewrite ++-assoc l' (concat ls) l | concat-foldr ls l = refl

--concat-foldr (l' :: (l'' :: ls)) l rewrite ++-assoc l' (concat (l'' :: ls)) l | concat-foldr (l'' :: ls) l = refl

longer-trans : âˆ€{â„“}{A : Set â„“}(l1 l2 l3 : ğ•ƒ A) â†’ 
                l1 longer l2 â‰¡ tt â†’
                l2 longer l3 â‰¡ tt â†’
                l1 longer l3 â‰¡ tt
longer-trans [] l2 l3 () q 
longer-trans (x :: l1) [] l3 p ()
longer-trans (x :: l1) (xâ‚ :: l2) [] p q = refl
longer-trans (x :: l1) (xâ‚ :: l2) (xâ‚‚ :: l3) p q = longer-trans l1 l2 l3 p q

filter-idem : âˆ€{â„“}{A : Set â„“}(p : A â†’ ğ”¹)(l : ğ•ƒ A) â†’
              (filter p (filter p l)) â‰¡ (filter p l)
filter-idem p [] = refl
filter-idem p (x :: l) with keep (p x)
filter-idem p (x :: l) | tt , p' = cont p'
  where h : p x â‰¡ tt â†’ (if p x then x :: filter p l else filter p l) â‰¡ x :: filter p l
        h u rewrite u = refl
        cont : p x â‰¡ tt â†’ filter p (if p x then x :: filter p l else filter p l) â‰¡
                            (if p x then x :: filter p l else filter p l)
        cont u rewrite h u | u | filter-idem p l = refl
filter-idem p (x :: l) | ff , p' rewrite p' = filter-idem p l

length-filter : âˆ€{â„“}{A : Set â„“}(p : A â†’ ğ”¹)(l : ğ•ƒ A) â†’ 
                length (filter p l) â‰¤ length l â‰¡ tt
length-filter p [] = refl
length-filter p (x :: l) with p x
length-filter p (x :: l) | tt = length-filter p l
length-filter p (x :: l) | ff = 
  â‰¤-trans{length (filter p l)} (length-filter p l) (â‰¤-suc (length l))

filter-++ : âˆ€{â„“}{A : Set â„“}(p : A â†’ ğ”¹)(l1 l2 : ğ•ƒ A) â†’ filter p (l1 ++ l2) â‰¡ filter p l1 ++ filter p l2
filter-++ p [] l2 = refl
filter-++ p (x :: l1) l2 with p x 
filter-++ p (x :: l1) l2 | tt rewrite (filter-++ p l1 l2) = refl
filter-++ p (x :: l1) l2 | ff rewrite (filter-++ p l1 l2) = refl

remove-++ : âˆ€{â„“}{A : Set â„“}(eq : A â†’ A â†’ ğ”¹)(a : A)(l1 l2 : ğ•ƒ A) â†’ 
            remove eq a (l1 ++ l2) â‰¡ remove eq a l1 ++ remove eq a l2
remove-++ eq a l1 l2 = filter-++ (Î» x â†’ ~ (eq a x)) l1 l2

::-injective : âˆ€{â„“}{A : Set â„“}{x y : A}{xs ys : ğ•ƒ A} â†’ 
               x :: xs â‰¡ y :: ys â†’ x â‰¡ y âˆ§ xs â‰¡ ys
::-injective refl = refl , refl

concat-++ : âˆ€{â„“}{A : Set â„“}(ls1 ls2 : ğ•ƒ (ğ•ƒ A)) â†’ concat (ls1 ++ ls2) â‰¡ (concat ls1) ++ (concat ls2)
concat-++ [] ls2 = refl
concat-++ (l :: ls) ls2 rewrite concat-++ ls ls2 = sym (++-assoc l (concat ls) (concat ls2))

-- This holds as long as we have the equations pâ‚ and pâ‚‚.  We know
-- that these equations are consistant to adopt, because they are
-- equivalent up and an isomorphism, and hence, by univalence they are
-- consistent as equations.  The respective isomorphisms can be found
-- in products-thms.agda.
all-pred-append : âˆ€{X : Set}{f : X â†’ Set}{lâ‚ lâ‚‚}
  â†’ (pâ‚ : âˆ€{â„“}{A : Set â„“} â†’ A â‰¡ (âŠ¤ âˆ§ A))
  â†’ (pâ‚‚ : âˆ€{â„“}{A B C : Set â„“} â†’  (A âˆ§ (B âˆ§ C)) â‰¡ ((A âˆ§ B) âˆ§ C))
  â†’ all-pred f (lâ‚ ++ lâ‚‚) â‰¡ ((all-pred f lâ‚) âˆ§ (all-pred f lâ‚‚))
all-pred-append {lâ‚ = []} {lâ‚‚} pâ‚ pâ‚‚ = pâ‚
all-pred-append {X}{f}{x :: lâ‚} {lâ‚‚} pâ‚ pâ‚‚ rewrite all-pred-append {X}{f}{lâ‚ = lâ‚} {lâ‚‚} pâ‚ pâ‚‚ = pâ‚‚ 

map-proj-âŠâ‚ : âˆ€{â„“ â„“'}{A : Set â„“}{B : Set â„“'} â†’ (l : ğ•ƒ A) â†’ 
                proj-âŠâ‚ {A = A}{B} (map injâ‚ l) â‰¡ l
map-proj-âŠâ‚ [] = refl
map-proj-âŠâ‚ {A = A}{B} (x :: l) rewrite map-proj-âŠâ‚ {A = A}{B} l = refl

map-proj-âŠâ‚‚ : âˆ€{â„“ â„“'}{A : Set â„“}{B : Set â„“'} â†’ (l : ğ•ƒ B) â†’ 
                proj-âŠâ‚‚ {A = A}{B} (map injâ‚‚ l) â‰¡ l
map-proj-âŠâ‚‚ [] = refl
map-proj-âŠâ‚‚ {A = A}{B} (x :: l) rewrite map-proj-âŠâ‚‚ {A = A}{B} l = refl

map-proj-âŠâ‚‚-[] : âˆ€{â„“ â„“'}{A : Set â„“}{B : Set â„“'} â†’ (l : ğ•ƒ A) â†’ 
                  proj-âŠâ‚‚ {A = A}{B} (map injâ‚ l) â‰¡ []
map-proj-âŠâ‚‚-[] [] = refl
map-proj-âŠâ‚‚-[] {A = A}{B} (x :: l) rewrite map-proj-âŠâ‚‚-[] {A = A}{B} l = refl

map-proj-âŠâ‚-[] : âˆ€{â„“ â„“'}{A : Set â„“}{B : Set â„“'} â†’ (l : ğ•ƒ B) â†’ 
                  proj-âŠâ‚ {A = A}{B} (map injâ‚‚ l) â‰¡ []
map-proj-âŠâ‚-[] [] = refl
map-proj-âŠâ‚-[] {A = A}{B} (x :: l) rewrite map-proj-âŠâ‚-[] {A = A}{B} l = refl

is-empty-++ : âˆ€{â„“}{A : Set â„“}(l1 l2 : ğ•ƒ A) â†’ is-empty (l1 ++ l2) â‰¡ is-empty l1 && is-empty l2
is-empty-++ [] l2 = refl
is-empty-++ (x :: l1) l2 = refl

is-empty-ff-length : âˆ€{â„“}{A : Set â„“}(l : ğ•ƒ A) â†’ is-empty l â‰¡ ff â†’ length l =â„• 0 â‰¡ ff
is-empty-ff-length [] ()
is-empty-ff-length (x :: l) p = refl
