module nat-thms where

open import bool
open import bool-thms
open import bool-thms2
open import eq
open import nat
open import neq
open import product
open import product-thms
open import sum

--------------------------------------------------
-- properties of addition
--------------------------------------------------

0+ : âˆ€ (x : â„•) â†’ 0 + x â‰¡ x
0+ x = refl

+0 : âˆ€ (x : â„•) â†’ x + 0 â‰¡ x
+0 zero = refl
+0 (suc x) rewrite +0 x = refl

+1 : âˆ€ (x : â„•) â†’ x + 1 â‰¡ suc x
+1 zero = refl
+1 (suc x) rewrite +1 x = refl

+suc : âˆ€ (x y : â„•) â†’ x + (suc y) â‰¡ suc(x + y)
+suc zero y = refl
+suc (suc x) y rewrite +suc x y = refl

+assoc : âˆ€ (x y z : â„•) â†’ x + (y + z) â‰¡ (x + y) + z
+assoc zero y z = refl
+assoc (suc x) y z rewrite +assoc x y z = refl

+comm : âˆ€ (x y : â„•) â†’ x + y â‰¡ y + x
+comm zero y rewrite +0 y = refl
+comm (suc x) y rewrite +suc y x | +comm x y = refl

+perm : âˆ€ (x y z : â„•) â†’ x + (y + z) â‰¡ y + (x + z)
+perm x y z rewrite +assoc x y z | +comm x y | sym (+assoc y x z) = refl

+perm2 : âˆ€ (x y z : â„•) â†’ (x + y) + z â‰¡ (x + z) + y
+perm2 x y z rewrite sym (+assoc x y z) | +comm y z | +assoc x z y = refl

+â‰¡0 : âˆ€ {x y : â„•} â†’ x + y â‰¡ 0 â†’ x â‰¡ 0 âˆ§ y â‰¡ 0
+â‰¡0{zero}{zero} p = refl , refl
+â‰¡0{zero}{suc y} ()
+â‰¡0{suc x}{zero} ()
+â‰¡0{suc x}{suc y} ()

--------------------------------------------------
-- properties of multiplication
--------------------------------------------------

*0 : âˆ€ (x : â„•) â†’ x * 0 â‰¡ 0
*0 zero = refl
*0 (suc x) rewrite *0 x = refl

*1 : âˆ€ {n : â„•} â†’ n * 1 â‰¡ n
*1 {0} = refl
*1 {suc n} rewrite *1 {n} = refl

*suc : âˆ€ (x y : â„•) â†’ x * (suc y) â‰¡ x + x * y
*suc zero y = refl
*suc (suc x) y rewrite *suc x y | +assoc y x (x * y) | +assoc x y (x * y) | +comm y x = refl

*distribr : âˆ€ (x y z : â„•) â†’ (x + y) * z â‰¡ x * z + y * z
*distribr zero y z = refl
*distribr (suc x) y z rewrite *distribr x y z = +assoc z (x * z) (y * z) 

*distribl : âˆ€ (x y z : â„•) â†’ x * (y + z) â‰¡ x * y + x * z
*distribl 0 y z = refl
*distribl (suc x) y z rewrite *distribl x y z | +assoc (y + z) (x * y) (x * z) | +assoc (y + x * y) z (x * z) | +comm (y + z) (x * y) | +assoc (x * y) y z | +comm (x * y) y = refl

*comm : âˆ€ (x y : â„•) â†’ x * y â‰¡ y * x
*comm zero y rewrite *0 y = refl
*comm (suc x) y rewrite *suc y x | *comm x y = refl

*assoc : âˆ€ (x y z : â„•) â†’ x * (y * z) â‰¡ (x * y) * z
*assoc zero y z = refl
*assoc (suc x) y z rewrite *assoc x y z | *distribr y (x * y) z = refl

--------------------------------------------------
-- basic properties of pred
--------------------------------------------------

sucpred : âˆ€ {x : â„•} â†’ iszero x â‰¡ ff â†’ suc (pred x) â‰¡ x
sucpred{0} ()
sucpred{suc x} p = refl

pred+ : âˆ€ (x y : â„•) â†’ iszero x â‰¡ ff â†’ (pred x) + y â‰¡ pred (x + y)
pred+ 0 y ()
pred+ (suc x) y p = refl

--------------------------------------------------
-- properties of <, â‰¤, and =â„•, iszero
--------------------------------------------------

<-0 : âˆ€ (x : â„•) â†’ x < 0 â‰¡ ff
<-0 0 = refl
<-0 (suc y) = refl

0-â‰¤ : âˆ€ (x : â„•) â†’ 0 â‰¤ x â‰¡ tt
0-â‰¤ 0 = refl
0-â‰¤ (suc x) = refl

<-drop : âˆ€ {x y : â„•} â†’ (x < (suc y) â‰¡ tt) â†’ x â‰¡ y âˆ¨ x < y â‰¡ tt
<-drop {0} {0} p = injâ‚ refl
<-drop {suc x} {0} p rewrite <-0 x = ð”¹-contra p
<-drop {0} {suc y} p = injâ‚‚ refl
<-drop {suc x} {suc y} p with <-drop {x} {y} p 
... | injâ‚ u rewrite u = injâ‚ refl
... | injâ‚‚ u = injâ‚‚ u

=â„•-refl : âˆ€ (x : â„•) â†’ (x =â„• x) â‰¡ tt
=â„•-refl 0 = refl
=â„•-refl (suc x) = (=â„•-refl x)

=â„•-to-â‰¡ : âˆ€ {x y : â„•} â†’ x =â„• y â‰¡ tt â†’ x â‰¡ y
=â„•-to-â‰¡ {0} {0} u = refl
=â„•-to-â‰¡ {suc x} {0} ()
=â„•-to-â‰¡ {0} {suc y} ()
=â„•-to-â‰¡ {suc x} {suc y} u rewrite =â„•-to-â‰¡ {x} {y} u = refl

=â„•-from-â‰¡ : âˆ€ {x y : â„•} â†’ x â‰¡ y â†’ x =â„• y â‰¡ tt
=â„•-from-â‰¡ {x} refl = =â„•-refl x

=â„•-sym : âˆ€ (x y : â„•) â†’ (x =â„• y) â‰¡ (y =â„• x)
=â„•-sym 0 0 = refl
=â„•-sym 0 (suc y) = refl
=â„•-sym (suc x) 0 = refl
=â„•-sym (suc x) (suc y) rewrite =â„•-sym x y = refl

=â„•-suc : âˆ€ (x : â„•) â†’ suc x =â„• x â‰¡ ff
=â„•-suc 0 = refl
=â„•-suc (suc x) = =â„•-suc x

<-suc : âˆ€ (n : â„•) â†’ n < suc n â‰¡ tt
<-suc 0 = refl
<-suc (suc n) rewrite <-suc n = refl

<-suc2 : âˆ€ (n : â„•) â†’ suc n < n â‰¡ ff
<-suc2 0 = refl
<-suc2 (suc n) = <-suc2 n

â‰¤-suc : âˆ€ (n : â„•) â†’ n â‰¤ suc n â‰¡ tt
â‰¤-suc n rewrite <-suc n = refl

â‰¤-suc2 : âˆ€ (n : â„•) â†’ suc n â‰¤ n â‰¡ ff
â‰¤-suc2 n rewrite <-suc2 n | =â„•-suc n = refl

<-push : âˆ€ {x y : â„•} â†’ (suc x) < y â‰¡ tt â†’ Î£ â„• (Î» y' â†’ y â‰¡ (suc y'))
<-push {x} {0} ()
<-push {0} {suc y} p = (y , refl)
<-push {suc x} {suc y} p with <-push {x} {y} p 
... | ( y' , p' ) rewrite p' = (suc y' , refl)

suc-inj : âˆ€ {n m : â„•} â†’ suc n â‰¡ suc m â†’ n â‰¡ m
suc-inj {n} {m} p rewrite (=â„•-to-â‰¡{n} (=â„•-from-â‰¡ p)) = refl

<-implies-suc : âˆ€ {x y : â„•} â†’ x < y â‰¡ tt â†’ Î£ â„• Î» y' â†’ y â‰¡ suc y'
<-implies-suc{x}{0} p rewrite <-0 x = ð”¹-contra p
<-implies-suc{y = suc y} p = y , refl

<=â„•ff : âˆ€ (x : â„•) â†’ 0 < x â‰¡ tt â†’ x =â„• 0 â‰¡ ff
<=â„•ff 0 ()
<=â„•ff (suc x) p = refl

nonzero< : âˆ€ {n : â„•} â†’ iszero n â‰¡ ff â†’ 0 < n â‰¡ tt
nonzero<{0} ()
nonzero<{(suc n)} p = refl

iszerosum : âˆ€ (x y : â„•) â†’ iszero(x + y) â‰¡ iszero(x) && iszero(y)
iszerosum 0 y = refl
iszerosum (suc x) y = refl

iszerosum2 : âˆ€ (x y : â„•) â†’ iszero x â‰¡ ff â†’ iszero(x + y) â‰¡ ff
iszerosum2 0 y ()
iszerosum2 (suc x) y _ = refl

iszeromult : âˆ€ (x y : â„•) â†’ iszero x â‰¡ ff â†’ iszero y â‰¡ ff â†’ 
               iszero (x * y) â‰¡ ff
iszeromult zero zero () q 
iszeromult zero (suc y) () q
iszeromult (suc x) zero p ()
iszeromult (suc x) (suc y) p q = refl

<â‰¤ : âˆ€ {n m : â„•} â†’ n < m â‰¡ tt â†’ n â‰¤ m â‰¡ tt
<â‰¤ {n}{m} p rewrite p = refl

â‰¤+1 : âˆ€(x y : â„•) â†’ x â‰¤ x + y â‰¡ tt
â‰¤+1 zero zero = refl
â‰¤+1 zero (suc y) = refl
â‰¤+1 (suc x) zero rewrite +0 x | =â„•-refl x | ||-tt (x < x) = refl
â‰¤+1 (suc x) (suc y) = â‰¤+1 x (suc y)

â‰¤+2 : âˆ€(x y : â„•) â†’ y â‰¤ x + y â‰¡ tt
â‰¤+2 x y rewrite +comm x y = â‰¤+1 y x

-- a theorem about quotients q, divisors d, and remainders r
Ã·< : âˆ€ {d q r x : â„•} â†’ 1 < d â‰¡ tt â†’ q * d + r â‰¡ suc x â†’ q < suc x â‰¡ tt
Ã·<{0} () p
Ã·<{suc 0} () p
Ã·<{suc (suc d)}{0} u p = refl
Ã·<{suc (suc d)}{suc q}{r}{0} u ()
Ã·<{suc (suc d)}{suc q}{r}{suc x} u p with suc-inj{suc (d + q * suc (suc d) + r)}{suc x} p
... | p' rewrite sym (+suc (d + q * suc (suc d)) r) | +comm d (q * suc (suc d)) 
               | sym (+assoc (q * (suc (suc d))) d (suc r)) = Ã·<{suc (suc d)}{q}{d + suc r}{x} refl p'  

--------------------------------------------------
-- ordering properties of < and â‰¤â„•
--------------------------------------------------

<-irrefl : âˆ€ (n : â„•) â†’ n < n â‰¡ ff
<-irrefl 0 = refl
<-irrefl (suc n) = <-irrefl n

<-asym : âˆ€ {x y : â„•} â†’ x < y â‰¡ tt â†’ y < x â‰¡ ff
<-asym {0} {0} _ = refl
<-asym {0} {suc y} p = refl
<-asym {suc x}{0} ()
<-asym {suc x}{suc y} p = <-asym {x} {y} p

â„•-trichotomyð”¹ : âˆ€ (n m : â„•) â†’ n < m || n =â„• m || m < n â‰¡ tt
â„•-trichotomyð”¹ 0 0 = refl
â„•-trichotomyð”¹ 0 (suc m) = refl
â„•-trichotomyð”¹ (suc n) 0 = refl
â„•-trichotomyð”¹ (suc n) (suc m) = â„•-trichotomyð”¹ n m

â„•-trichotomy : âˆ€ (n m : â„•) â†’ (n < m â‰¡ tt) âˆ¨ (n =â„• m â‰¡ tt) âˆ¨ (m < n â‰¡ tt)
â„•-trichotomy n m with ||-split{n < m} (â„•-trichotomyð”¹ n m)
... | injâ‚ p = injâ‚ p
... | injâ‚‚ p with ||-split{n =â„• m} p
... | injâ‚ p' = injâ‚‚ (injâ‚ p')
... | injâ‚‚ p' = injâ‚‚ (injâ‚‚ p')

<-insert : âˆ€ {x n m : â„•} â†’ n â‰¤ m â‰¡ tt â†’ (x < n â‰¡ tt) âˆ¨ (n â‰¤ x && x â‰¤ m â‰¡ tt) âˆ¨ (m < x â‰¡ tt)
<-insert{x}{n}{m} q with â„•-trichotomy x n
<-insert{x}{n}{m} q | injâ‚ p = injâ‚ p
<-insert{x}{n}{m} q | injâ‚‚ (injâ‚ p) rewrite (=â„•-to-â‰¡{x} p) | =â„•-refl n | ||-tt (n < n) = injâ‚‚ (injâ‚ q)
<-insert{x}{n}{m} q | injâ‚‚ (injâ‚‚ p) rewrite p with â„•-trichotomy x m
<-insert{x}{n}{m} q | injâ‚‚ (injâ‚‚ p) | injâ‚ p' rewrite p' = injâ‚‚ (injâ‚ refl)
<-insert{x}{n}{m} q | injâ‚‚ (injâ‚‚ p) | injâ‚‚ (injâ‚ p') rewrite p' | ||-tt (x < m) = injâ‚‚ (injâ‚ refl)
<-insert{x}{n}{m} q | injâ‚‚ (injâ‚‚ p) | injâ‚‚ (injâ‚‚ p') = injâ‚‚ (injâ‚‚ p')

<-insert2 : âˆ€ {x n m : â„•} â†’ n â‰¤ m â‰¡ tt â†’ (x < n â‰¡ tt) âˆ¨ (n â‰¤ x â‰¡ tt âˆ§ x â‰¤ m â‰¡ tt) âˆ¨ (m < x â‰¡ tt)
<-insert2{x}{n}{m} p with <-insert{x}{n}{m} p
<-insert2{x}{n}{m} p | injâ‚ p' = injâ‚ p'
<-insert2{x}{n}{m} p | injâ‚‚ (injâ‚ p') with &&-elim {n â‰¤ x} {x â‰¤ m} p'
<-insert2{x}{n}{m} p | injâ‚‚ (injâ‚ p') | p1 , p2 = injâ‚‚ (injâ‚ (p1 , p2))
<-insert2{x}{n}{m} p | injâ‚‚ (injâ‚‚ p') = injâ‚‚ (injâ‚‚ p')

<-trans : âˆ€ {x y z : â„•} â†’ x < y â‰¡ tt â†’ y < z â‰¡ tt â†’ x < z â‰¡ tt
<-trans {x} {0} p1 p2 rewrite <-0 x = ð”¹-contra p1
<-trans {0} {suc y} {0} p1 () 
<-trans {0} {suc y} {suc z} p1 p2 = refl
<-trans {suc x} {suc y} {0} p1 () 
<-trans {suc x} {suc y} {suc z} p1 p2 = <-trans {x} {y} {z} p1 p2

<â‰¤-trans : âˆ€ {x y z : â„•} â†’ x < y â‰¡ tt â†’ y â‰¤ z â‰¡ tt â†’ x < z â‰¡ tt
<â‰¤-trans {x} {y} {z} p1 p2 with ||-split p2
... | injâ‚ p' = <-trans{x}  p1 p'
... | injâ‚‚ p' rewrite =â„•-to-â‰¡ {y} {z} p' = p1

â‰¤<-trans : âˆ€ {x y z : â„•} â†’ x â‰¤ y â‰¡ tt â†’ y < z â‰¡ tt â†’ x < z â‰¡ tt
â‰¤<-trans {x} {y} {z} p1 p2 with ||-split p1
... | injâ‚ p' = <-trans{x} p' p2
... | injâ‚‚ p' rewrite =â„•-to-â‰¡ {x} {y} p' = p2

â‰¤-refl : âˆ€ (x : â„•) â†’ x â‰¤ x â‰¡ tt
â‰¤-refl 0 = refl
â‰¤-refl (suc x) = â‰¤-refl x

â‰¤-trans : âˆ€ {x y z : â„•} â†’ x â‰¤ y â‰¡ tt â†’ y â‰¤ z â‰¡ tt â†’ x â‰¤ z â‰¡ tt
â‰¤-trans {x} {y} {z} p1 p2 with ||-split p1 | ||-split p2
... | injâ‚ p' | injâ‚ p'' rewrite <-trans {x} p' p'' = refl
... | injâ‚‚ p' | injâ‚ p'' rewrite =â„•-to-â‰¡ {x} p'  | p'' = refl
... | injâ‚ p' | injâ‚‚ p'' rewrite =â„•-to-â‰¡ {y} p'' | p' = refl
... | injâ‚‚ p' | injâ‚‚ p'' rewrite =â„•-to-â‰¡ {x} p'  | =â„•-to-â‰¡ {y} p'' | =â„•-refl z | ||-tt (z < z) = refl

sucâ‰¤ : âˆ€ {n n' : â„•} â†’ suc n â‰¤ suc n' â‰¡ tt â†’ n â‰¤ n' â‰¡ tt
sucâ‰¤{n}{n'} p = p

sucâ‰¤< : âˆ€ {n n' : â„•} â†’ suc n â‰¤ n' â‰¡ tt â†’ n < n' â‰¡ tt
sucâ‰¤<{n} p = <â‰¤-trans{n} (<-suc n) p 

suc<< : âˆ€ {n' n : â„•} â†’ suc n < n' â‰¡ tt â†’ n < n' â‰¡ tt
suc<<{n = n} p = <-trans{n} (<-suc n) p 

<-suc-trans : âˆ€{x y : â„•} â†’ x < y â‰¡ tt â†’ x < suc y â‰¡ tt
<-suc-trans{0}{0} _ = refl
<-suc-trans{suc x}{0} ()
<-suc-trans{0}{suc y} _ = refl
<-suc-trans{suc x}{suc y} p = <-suc-trans{x}{y} p

â‰¤-suc-trans : âˆ€{x y : â„•} â†’ x â‰¤ y â‰¡ tt â†’ x â‰¤ suc y â‰¡ tt
â‰¤-suc-trans{0}{0} _ = refl
â‰¤-suc-trans{suc x}{0} ()
â‰¤-suc-trans{0}{suc y} _ = refl
â‰¤-suc-trans{suc x}{suc y} p = â‰¤-suc-trans{x}{y} p

-------------------------------------------------------------
-- more properties relating <, â‰¤ with arithmetic operations
-------------------------------------------------------------

<+ : âˆ€ {x y : â„•} â†’ y =â„• 0 â‰¡ ff â†’ x < y + x â‰¡ tt
<+{y = 0} ()
<+{x}{suc 0} p = <-suc x
<+{x}{suc (suc y)} p = <-trans{x}{(suc y) + x}{suc ((suc y) + x)} (<+{x}{suc y} refl) (<-suc ((suc y) + x))

<+2 : âˆ€ {x y : â„•} â†’ x < (suc y) + x â‰¡ tt
<+2{x}{y} = <+{x}{suc y} refl

<-iter-suc-trans-t-h : (n : â„•) â†’ (x : â„•) â†’ (accum : â„•) â†’ Set
<-iter-suc-trans-t-h 0 x accum = x < accum â‰¡ tt
<-iter-suc-trans-t-h (suc n) x accum = <-iter-suc-trans-t-h n x (suc accum)

<-iter-suc-trans-t : (n : â„•) â†’ (x : â„•) â†’ Set
<-iter-suc-trans-t n x = <-iter-suc-trans-t-h n x (suc x)

<-iter-suc-trans-h : âˆ€ (n : â„•) â†’ (x : â„•) â†’ (accum : â„•) â†’ x < accum â‰¡ tt â†’ <-iter-suc-trans-t-h n x accum
<-iter-suc-trans-h 0 x accum p = p
<-iter-suc-trans-h (suc n) x accum p = <-iter-suc-trans-h n x (suc accum) (<-suc-trans{x} p)

<-iter-suc-trans : âˆ€ (n : â„•) â†’ (x : â„•) â†’ <-iter-suc-trans-t n x
<-iter-suc-trans n x = <-iter-suc-trans-h n x (suc x) (<-suc x)

â‰¤0 : âˆ€ (n : â„•) â†’ 0 â‰¤ n â‰¡ tt
â‰¤0 0 = refl
â‰¤0 (suc n) = refl

â‰¤2* : âˆ€ (x : â„•) â†’ x â‰¤ 2 * x â‰¡ tt
â‰¤2* 0 = refl
â‰¤2* (suc x) rewrite +suc x (x + 0) | â‰¤<-trans {x} (â‰¤2* x) (<-suc (2 * x)) = refl

0<+ : âˆ€ (x y : â„•) â†’ 0 < y â‰¡ tt â†’ 0 < x + y â‰¡ tt
0<+ 0 y p = p
0<+ (suc x) y p = refl

<=â„•ff2 : âˆ€ (x : â„•) â†’ 1 < x â‰¡ tt â†’ x =â„• 0 â‰¡ ff
<=â„•ff2 x p = <=â„•ff x (<-trans{0}{1}{x} refl p)

*â‰¤ : âˆ€(x y : â„•) â†’ x â‰¤ x * (suc y) â‰¡ tt
*â‰¤ zero y = refl
*â‰¤ (suc x) y = â‰¤-trans {x} (*â‰¤ x y) (â‰¤+2 y (x * suc y))

--------------------------------------------------
-- relationships between â‰¤ and <
--------------------------------------------------

â‰¤ff : âˆ€ {x y : â„•} â†’ x â‰¤ y â‰¡ ff â†’ y < x â‰¡ tt
â‰¤ff{0}{0} ()
â‰¤ff{0}{suc y} ()
â‰¤ff{suc x}{0} _ = refl
â‰¤ff{suc x}{suc y} p rewrite â‰¤ff {x}{y} p = refl

<ff : âˆ€ {x y : â„•} â†’ x < y â‰¡ ff â†’ y â‰¤ x â‰¡ tt
<ff{x}{y} p with â„•-trichotomy x y
... | injâ‚ u rewrite u = ð”¹-contra (sym p)
... | injâ‚‚ (injâ‚ u) rewrite (=â„•-to-â‰¡{x} u) | =â„•-refl y | ||-tt (y < y) = refl
... | injâ‚‚ (injâ‚‚ u) rewrite u = refl

<-not-=â„• : âˆ€{x y : â„•} â†’ x < y â‰¡ tt â†’ y =â„• x â‰¡ ff
<-not-=â„•{0}{0} ()
<-not-=â„•{suc x}{0} ()
<-not-=â„•{0}{suc y} p = refl
<-not-=â„•{suc x}{suc y} p = <-not-=â„•{x}{y} p

<-not-> : âˆ€{x y : â„•} â†’ x < y â‰¡ tt â†’ y < x â‰¡ ff
<-not->{0}{0} ()
<-not->{suc x}{0} ()
<-not->{0}{suc y} p = refl
<-not->{suc x}{suc y} p = <-not->{x}{y} p

<tt : âˆ€ {x y : â„•} â†’ x < y â‰¡ tt â†’ y â‰¤ x â‰¡ ff
<tt{x}{y} p rewrite <-not-=â„•{x}{y} p | <-not->{x}{y} p = refl

â‰¤-antisym : âˆ€{x y : â„•} â†’ x â‰¤ y â‰¡ tt â†’ y â‰¤ x â‰¡ tt â†’ x â‰¡ y
â‰¤-antisym{x}{y} p q with ||-split {x < y} p 
â‰¤-antisym{x}{y} p q | injâ‚ u rewrite <tt{x} u with q
â‰¤-antisym{x}{y} p q | injâ‚ u | ()
â‰¤-antisym{x}{y} p q | injâ‚‚ u = =â„•-to-â‰¡ u

--------------------------------------------------
-- monotonicity properties of < and â‰¤â„•
--------------------------------------------------
<+mono1 : âˆ€ {z x y : â„•} â†’ x < y â‰¡ tt â†’ z + x < z + y â‰¡ tt
<+mono1{0} p = p
<+mono1{suc z} p = <+mono1{z} p

<+mono2 : âˆ€ {x y z : â„•} â†’ x < y â‰¡ tt â†’ x + z < y + z â‰¡ tt
<+mono2{x}{y}{z} p rewrite +comm x z | +comm y z | <+mono1{z}{x}{y} p = refl

--------------------------------------------------
-- properties of subtraction
--------------------------------------------------

0âˆ¸ : âˆ€ {x : â„•} â†’ 0 âˆ¸ x â‰¡ 0
0âˆ¸{0} = refl
0âˆ¸{suc x} = refl

âˆ¸â‰¤ : âˆ€ (x y : â„•) â†’ x âˆ¸ y â‰¤ x â‰¡ tt
âˆ¸â‰¤ 0 0 = refl
âˆ¸â‰¤ (suc x) 0 rewrite (=â„•-refl x) = ||-tt (x < x)
âˆ¸â‰¤ 0 (suc y) = refl
âˆ¸â‰¤ (suc x) (suc y) with ||-split{x âˆ¸ y < x}{x âˆ¸ y =â„• x} (âˆ¸â‰¤ x y)
... | injâ‚ u rewrite <-trans {x âˆ¸ y} u (<-suc x) = refl
... | injâ‚‚ u rewrite (=â„•-to-â‰¡ {x âˆ¸ y} u) | <-suc x = refl

âˆ¸< : âˆ€ {x y : â„•} â†’ x =â„• 0 â‰¡ ff â†’ x âˆ¸ (suc y) < x â‰¡ tt
âˆ¸< {0} {y} ()
âˆ¸< {suc x} {y} _ with ||-split{x âˆ¸ y < x}{x âˆ¸ y =â„• x} (âˆ¸â‰¤ x y) 
... | injâ‚ u = <-trans {x âˆ¸ y} u (<-suc x)
... | injâ‚‚ u rewrite (=â„•-to-â‰¡ {x âˆ¸ y} u) = <-suc x

âˆ¸<1 : âˆ€ {x y : â„•} â†’ x âˆ¸ y < suc x â‰¡ tt
âˆ¸<1 {zero} {zero} = refl
âˆ¸<1 {zero} {suc y} = refl
âˆ¸<1 {suc x} {zero} = <-suc x
âˆ¸<1 {suc x} {suc y} = <-trans {x âˆ¸ y}{suc x} (âˆ¸<1 {x} {y}) (<-suc x)

+âˆ¸1 : âˆ€ {x y : â„•} â†’ x < y â‰¡ tt â†’ x + (y âˆ¸ x) â‰¡ y
+âˆ¸1{0} p = refl
+âˆ¸1{suc x}{0} ()
+âˆ¸1{suc x}{suc y} p rewrite +âˆ¸1{x}{y} p = refl

âˆ¸+ : âˆ€ {x y z : â„•} â†’ x âˆ¸ (y + z) â‰¡ (x âˆ¸ y) âˆ¸ z
âˆ¸+{x}{0} = refl
âˆ¸+{0}{suc y}{z} rewrite 0âˆ¸{z} = refl
âˆ¸+{suc x}{suc y} = âˆ¸+{x}{y}

âˆ¸+2 : âˆ€ {x y : â„•} â†’ y â‰¤ x â‰¡ tt â†’ (x âˆ¸ y) + y â‰¡ x
âˆ¸+2{0}{0} _ = refl
âˆ¸+2{suc x}{0} _ rewrite +0 x = refl
âˆ¸+2{0}{suc y} ()
âˆ¸+2{suc x}{suc y} p rewrite +suc (x âˆ¸ y) y | âˆ¸+2{x}{y} p = refl

âˆ¸eq-swap : âˆ€ {x y z : â„•} â†’ y â‰¤ x â‰¡ tt â†’ z â‰¡ x âˆ¸ y â†’ z + y â‰¡ x
âˆ¸eq-swap{x}{y}{z} p q = lem (cong (Î» w â†’ w + y) q)
                        where lem : z + y â‰¡ (x âˆ¸ y) + y â†’ z + y â‰¡ x
                              lem p' rewrite âˆ¸+2{x}{y} p = p'

<âˆ¸ : âˆ€ {x y : â„•} â†’ (y < x â‰¡ tt) â†’ ((x âˆ¸ y =â„• 0) â‰¡ ff)
<âˆ¸ {0}{y} p with <-0 y 
... | q rewrite p = ð”¹-contra (sym q)
<âˆ¸ {suc x}{0} p = refl
<âˆ¸ {suc x}{suc y} p = <âˆ¸{x}{y} p

<âˆ¸suc : âˆ€ {x y : â„•} â†’ (y < x â‰¡ tt) â†’ Î£ â„• (Î» n â†’ x âˆ¸ y â‰¡ suc n)
<âˆ¸suc{x}{y} p with keep (x âˆ¸ y)
<âˆ¸suc{x}{y} p | 0 , r with <âˆ¸{x}{y} p
<âˆ¸suc{x}{y} p | 0 , r | q rewrite r with q
<âˆ¸suc{x}{y} p | 0 , r | q | ()
<âˆ¸suc{x}{y} p | suc n , r = n , r

âˆ¸suc : âˆ€ {x y z : â„• } â†’ y < x â‰¡ tt â†’ x âˆ¸ (y + (suc z)) < x âˆ¸ y â‰¡ tt
âˆ¸suc{x}{y}{z} p rewrite âˆ¸+{x}{y}{suc z} = âˆ¸< {x âˆ¸ y} (<âˆ¸{x}{y} p)

âˆ¸suc2 : âˆ€ {x y z : â„• } â†’ y < x â‰¡ tt â†’ x âˆ¸ ((suc z) + y) < x âˆ¸ y â‰¡ tt
âˆ¸suc2{x}{y}{z} p rewrite +comm (suc z) y = âˆ¸suc{x}{y}{z} p

âˆ¸cancel : âˆ€ (x y z : â„•) â†’ (x + y) âˆ¸ (x + z) â‰¡ y âˆ¸ z
âˆ¸cancel 0 y z = refl
âˆ¸cancel (suc x) y z = âˆ¸cancel x y z

distribr*âˆ¸ : âˆ€ (x y z : â„•) â†’ (x âˆ¸ y) * z â‰¡  x * z âˆ¸ y * z
distribr*âˆ¸ 0 y z rewrite 0âˆ¸{y} | 0âˆ¸{y * z} = refl
distribr*âˆ¸ (suc x) 0 z = refl
distribr*âˆ¸ (suc x) (suc y) z rewrite distribr*âˆ¸ x y z | âˆ¸cancel z (x * z) (y * z) = refl

âˆ¸â‰¤2 : âˆ€ (n x y : â„•) â†’  x â‰¤ suc n â‰¡ tt â†’ y =â„• 0 â‰¡ ff â†’ x âˆ¸ y â‰¤ n â‰¡ tt
âˆ¸â‰¤2 0 0 y p1 p2 rewrite 0âˆ¸{y} = refl
âˆ¸â‰¤2 0 (suc x) 0 p1 ()
âˆ¸â‰¤2 0 (suc 0) (suc y) p1 p2 rewrite 0âˆ¸{y}= refl
âˆ¸â‰¤2 0 (suc (suc x)) (suc y) () p2
âˆ¸â‰¤2 (suc n) 0 y p1 p2 rewrite 0âˆ¸{y} = refl
âˆ¸â‰¤2 (suc n) (suc x) 0 p1 ()
âˆ¸â‰¤2 (suc n) (suc x) (suc 0) p1 p2 = p1
âˆ¸â‰¤2 (suc n) (suc x) (suc (suc y)) p1 p2 = â‰¤-trans{x âˆ¸ suc y}{n}{suc n} (âˆ¸â‰¤2 n x (suc y) p1 refl) (â‰¤-suc n)

--------------------------------------------------
-- properties of min, max
--------------------------------------------------
min-forced1 : âˆ€ {n n' m : â„•} â†’ n < n' â‰¡ tt â†’ n â‰¡ min n' m â†’ n â‰¡ m
min-forced1{n}{n'}{m} p1 p2 with n' < m 
... | tt rewrite p2 = ð”¹-contra (trans (sym (<-irrefl n')) p1)
... | ff = p2

min-suc : âˆ€ (n m : â„•) â†’ min (suc n) (suc m) â‰¡ suc (min n m)
min-suc n m rewrite (ite-arg suc (n < m) n m) = refl

max-suc : âˆ€ (n m : â„•) â†’ max (suc n) (suc m) â‰¡ suc (max n m)
max-suc n m rewrite (ite-arg suc (n < m) m n) = refl

min-comm : âˆ€ (n m : â„•) â†’ min n m â‰¡ min m n
min-comm n m with â„•-trichotomy n m
... | injâ‚ p rewrite <-asym {n} p | p = refl
... | injâ‚‚ (injâ‚ p) rewrite =â„•-to-â‰¡ {n} p = refl
... | injâ‚‚ (injâ‚‚ p) rewrite <-asym {m} p | p = refl

min-same : âˆ€ (n : â„•) â†’ min n n â‰¡ n
min-same n rewrite <-irrefl n = refl

min-<1 : âˆ€ {n m : â„•} â†’ min n m â‰¤ m â‰¡ tt
min-<1{0}{0} = refl
min-<1{0}{suc m} = refl
min-<1{suc n}{0} = refl
min-<1{suc n}{suc m} rewrite min-suc n m = min-<1{n}

min-<2 : âˆ€ {n m : â„•} â†’ min n m â‰¤ n â‰¡ tt
min-<2{0}{0} = refl
min-<2{0}{suc m} = refl
min-<2{suc n}{0} = refl
min-<2{suc n}{suc m} rewrite min-suc n m = min-<2{n}

max-<1 : âˆ€ {n m : â„•} â†’ n â‰¤ max n m â‰¡ tt
max-<1{0}{0} = refl
max-<1{0}{suc m} = refl
max-<1{suc n}{0} rewrite =â„•-refl n | ||-tt (n < n) = refl
max-<1{suc n}{suc m} rewrite max-suc n m = max-<1{n}

max-<2 : âˆ€ {n m : â„•} â†’ n â‰¤ max n m â‰¡ tt
max-<2{0}{0} = refl
max-<2{0}{suc m} = refl
max-<2{suc n}{0} rewrite =â„•-refl n | ||-tt (n < n) = refl
max-<2{suc n}{suc m} rewrite max-suc n m = max-<2{n}

min-mono1 : âˆ€ (n n' m : â„•) â†’ n â‰¤ n' â‰¡ tt â†’ min n m â‰¤ min n' m â‰¡ tt
min-mono1 n n' m p with ||-split{n < n'} p 
... | injâ‚‚ p' rewrite =â„•-to-â‰¡ {n} p' | =â„•-refl (min n' m) | ||-tt ((min n' m) < (min n' m)) = refl
... | injâ‚ p' with â„•-trichotomy n' m
... | injâ‚ p'' rewrite <-trans {n} p' p'' | p'' | p' = refl
... | injâ‚‚ (injâ‚ p'') rewrite =â„•-to-â‰¡ {n'} p'' | <-irrefl m = min-<1{n}{m}
... | injâ‚‚ (injâ‚‚ p'') rewrite <-asym {m} p'' with â„•-trichotomy n m 
... | injâ‚ p''' rewrite min-<1{n}{m} = refl
... | injâ‚‚ (injâ‚ p''') rewrite =â„•-to-â‰¡ {n} p''' | <-irrefl m | =â„•-refl m | ||-tt (m < m) = refl
... | injâ‚‚ (injâ‚‚ p''') rewrite <-asym {m} p''' | =â„•-refl m | ||-tt (m < m) = refl

min-mono2 : âˆ€ (n m m' : â„•) â†’ m â‰¤ m' â‰¡ tt â†’ min n m â‰¤ min n m' â‰¡ tt
min-mono2 n m m' p rewrite min-comm n m | min-comm n m' = min-mono1 m m' n p

--------------------------------------------------
-- some disequalities
--------------------------------------------------

+â‰¢ : âˆ€ (x y : â„•) â†’ x â‰¢ x + suc y
+â‰¢ 0 y ()
+â‰¢ (suc x) y p with =â„•-from-â‰¡ {suc x} p
... | q with =â„•-to-â‰¡ {x} q 
... | r = +â‰¢ x y r

--------------------------------------------------
-- properties of parity
--------------------------------------------------
parity-even : âˆ€ (x : â„•) â†’ parity (x * 2) â‰¡ ff
parity-even 0 = refl
parity-even (suc x) rewrite parity-even x = refl

parity-even2 : âˆ€ (x : â„•) â†’ parity (2 * x) â‰¡ ff
parity-even2 x rewrite *comm 2 x = parity-even x

parity-odd : âˆ€ (x : â„•) â†’ parity (x * 2 + 1) â‰¡ tt
parity-odd 0 = refl
parity-odd (suc x) rewrite parity-odd x = refl

parity-add : âˆ€ (x y : â„•) â†’ parity (x + y) â‰¡ (parity x) xor (parity y)
parity-add 0 y rewrite ff-xor (parity y) = refl
parity-add (suc x) y rewrite parity-add x y | ~-xor-distrb (parity x) (parity y) = refl

parity-mult : âˆ€ (x y : â„•) â†’ parity (x * y) â‰¡ (parity x) && (parity y)
parity-mult 0 y = refl
parity-mult (suc x) y rewrite parity-add y (x * y) | parity-mult x y = xor-distrib-&& (parity y) (parity x)

--------------------------------------------------
-- properties of power
--------------------------------------------------
1-pow : âˆ€ {n : â„•} â†’ 1 pow n â‰¡ 1
1-pow {0} = refl
1-pow {(suc n)} rewrite 1-pow {n} = refl

nonzero-pow : âˆ€ (x y : â„•) â†’ x =â„• 0 â‰¡ ff â†’ iszero (x pow y) â‰¡ ff
nonzero-pow x 0 _ = refl
nonzero-pow 0 (suc y) ()
nonzero-pow (suc x) (suc y) p rewrite iszerosum2 (suc x pow y) (x * suc x pow y) (nonzero-pow (suc x) y refl) = refl

pow+ : âˆ€ (x y z : â„•) â†’ x pow (y + z) â‰¡ (x pow y) * (x pow z)
pow+ x 0 z rewrite +0 (x pow z) = refl
pow+ x (suc y) z rewrite pow+ x y z | *assoc x (x pow y) (x pow z) = refl

pow* : âˆ€ (x y z : â„•) â†’ x pow (y * z) â‰¡ (x pow y) pow z
pow* x y 0 rewrite *0 y = refl
pow* x y (suc z) rewrite sym (pow* x y z) | sym (pow+ x y (y * z)) | *comm y (suc z) | *comm y z = refl

--------------------------------------------------
-- properties of factorial
--------------------------------------------------
factorial-nonzero : âˆ€ (n : â„•) â†’ iszero (factorial n) â‰¡ ff
factorial-nonzero zero = refl
factorial-nonzero (suc x) rewrite iszerosum (factorial x) (x * factorial x) | factorial-nonzero x = refl

--------------------------------------------------
-- injectivity properties of addition
--------------------------------------------------
+inj1 : âˆ€ {x y z : â„•} â†’ x + y â‰¡ x + z â†’ y â‰¡ z
+inj1 {0} {y} {z} p = p
+inj1 {suc x} {y} {z} p = +inj1 {x} {y} {z} (suc-inj p)

+inj2 : âˆ€ {x y z : â„•} â†’ x + z â‰¡ y + z â†’ x â‰¡ y
+inj2 {x} {y} {z} p rewrite +comm x z | +comm y z = +inj1 {z} {x} {y} p

--------------------------------------------------
-- properties of is-even, is-odd
--------------------------------------------------

even~odd : âˆ€ (x : â„•) â†’ is-even x â‰¡ ~ is-odd x
odd~even : âˆ€ (x : â„•) â†’ is-odd x â‰¡ ~ is-even x
even~odd zero = refl
even~odd (suc x) = odd~even x
odd~even zero = refl
odd~even (suc x) = even~odd x
