module instances where
open import lib public renaming (return to returnáµ¢â‚’; _>>_ to _>>áµ¢â‚’_; _>>=_ to _>>=áµ¢â‚’_)
open import functions public


record functor {â„“ â„“'} (F : Set â„“ â†’ Set â„“') : Set (lsuc (â„“ âŠ” â„“')) where
  infixl 2 _<$>_ _<$_
  field
    fmap : âˆ€ {A B : Set â„“} â†’ (A â†’ B) â†’ F A â†’ F B

  {-functor-identity-law :
      âˆ€ {A} (fa : F A) â†’
        fmap id fa â‰¡ fa
    functor-composition-law :
      âˆ€ {A B C} (f : B â†’ C) (g : A â†’ B) (fa : F A) â†’
        fmap (f âˆ˜ g) fa â‰¡ fmap f (fmap g fa)-}
  
  _<$>_ = fmap

  _<$_ : âˆ€ {A B : Set â„“} â†’ A â†’ F B â†’ F A
  a <$ fb = (Î» _ â†’ a) <$> fb

open functor â¦ƒ...â¦„ public


record applicative {â„“ â„“'} (F : Set â„“ â†’ Set â„“') : Set (lsuc (â„“ âŠ” â„“')) where
  infixl 2 _<*>_ _<*_ _*>_
  field
    pure : âˆ€ {A : Set â„“} â†’ A â†’ F A
    _<*>_ : âˆ€ {A B : Set â„“} â†’ F (A â†’ B) â†’ F A â†’ F B
    â¦ƒ functorF â¦„ : functor F

  {-applicative-identity-law :
      âˆ€ {A} (v : F A) â†’
        pure id <*> v â‰¡ v
    applicative-composition-law :
      âˆ€ {A B C} (u : F (B â†’ C)) (v : F (A â†’ B)) (w : F A) â†’
        pure _âˆ˜_ <*> u <*> v <*> w â‰¡ u <*> (v <*> w)
    applicative-homomorphism-law :
      âˆ€ {A B} (f : A â†’ B) (x : A) â†’
        pure f <*> pure x â‰¡ pure (f x)
    applicative-interchange-law :
      âˆ€ {A B} (u : F (A â†’ B)) (y : A) â†’
        u <*> pure y â‰¡ pure (_$ y) <*> u-}
  
  _<*_ : âˆ€ {A B : Set â„“} â†’ F A â†’ F B â†’ F A
  fa <* fb = (Î» a b â†’ a) <$> fa <*> fb

  _*>_ : âˆ€ {A B : Set â„“} â†’ F A â†’ F B â†’ F B
  fa *> fb = (Î» a b â†’ b) <$> fa <*> fb

  liftA : âˆ€ {A B : Set â„“} â†’ (A â†’ B) â†’ F A â†’ F B
  liftA g fa = pure g <*> fa

  liftA2 : âˆ€ {A B C : Set â„“} â†’ (A â†’ B â†’ C) â†’ F A â†’ F B â†’ F C
  liftA2 g fa fb = pure g <*> fa <*> fb

  sequenceA : âˆ€ {A : Set â„“} â†’ ğ•ƒ (F A) â†’ F (ğ•ƒ A)
  sequenceA = foldr (liftA2 _::_) (pure [])

open applicative â¦ƒ...â¦„ public


record monad {â„“ â„“'} (F : Set â„“ â†’ Set â„“') : Set (lsuc (â„“ âŠ” â„“')) where
  infixr 2 _>>_ _>>=_ _=<<_ _>=>_ _>>=c_ _>>c_ _>>=?_ _>>=m_ _>>=s_ _>>=e_ _>>â‰ _ _>â‰¯_ _>>=r_ _>>r_

  field
    return : âˆ€{A : Set â„“} â†’ A â†’ F A
    _>>=_ : âˆ€{A B : Set â„“} â†’ F A â†’ (A â†’ F B) â†’ F B

  {-monad-left-identity-law :
      âˆ€ {A B} (a : A) (k : A â†’ F B) â†’
        return a >>= k â‰¡ k a
    monad-right-identity-law :
      âˆ€ {A} (m : F A) â†’
        m >>= return â‰¡ m
    monad-associativity-law :
      âˆ€ {A B C} (m : F A) (k : A â†’ F B) (h : B â†’ F C) â†’
        m >>= (Î» x â†’ k x >>= h) â‰¡ (m >>= k) >>= h-}

  _>>_ : âˆ€ {A B : Set â„“} â†’ F A â†’ F B â†’ F B
  fa >> fb = fa >>= Î» _ â†’ fb

  _=<<_ : âˆ€ {A B : Set â„“} â†’ (A â†’ F B) â†’ F A â†’ F B
  fab =<< fa = fa >>= fab
  
  _>=>_ : âˆ€ {A B C : Set â„“} â†’ (A â†’ F B) â†’ (B â†’ F C) â†’ (A â†’ F C)
  fab >=> fbc = Î» a â†’ fab a >>= fbc

  _>>=c_ : âˆ€ {A B C : Set â„“} â†’ F (A Ã— B) â†’ (A â†’ B â†’ F C) â†’ F C
  p >>=c f = p >>= Î» {(a , b) â†’ f a b}
  
  _>>c_ : âˆ€ {A B : Set â„“} â†’ F A â†’ F B â†’ F (A Ã— B)
  fa >>c fb = fa >>= Î» a â†’ fb >>= Î» b â†’ return (a , b)
  
  _>>=?_ : âˆ€ {A B : Set â„“} â†’ maybe (F A) â†’ (maybe A â†’ F B) â†’ F B
  nothing >>=? f = f nothing
  (just a) >>=? f = a >>= (f âˆ˜ just)

  _>>=s_ : âˆ€ {A B E : Set â„“} â†’ F (E âŠ A) â†’ (A â†’ F (E âŠ B)) â†’ F (E âŠ B)
  s >>=s f = s >>= Î» {(injâ‚ e) â†’ return (injâ‚ e); (injâ‚‚ a) â†’ f a}

  _>>=e_ : âˆ€ {A B : Set â„“} â†’ F (error-t A) â†’ (A â†’ F (error-t B)) â†’ F (error-t B)
  fe? >>=e f = fe? >>= Î» {(no-error a) â†’ f a; (yes-error e) â†’ return (yes-error e)}
  
  _>>=m_ : âˆ€{A B : Set â„“} â†’ F (maybe A) â†’ (A â†’ F (maybe B)) â†’ F (maybe B)
  m >>=m f = m >>= Î» {(just a) â†’ f a; nothing â†’ return nothing}

  _>>â‰ _  : âˆ€{A B : Set â„“} â†’ F A â†’ (A â†’ F B) â†’ F A
  (fâ‚ >>â‰  fâ‚‚) = fâ‚ >>= Î» result â†’ fâ‚‚ result >> return result

  _>â‰¯_ : âˆ€{A B : Set â„“} â†’ F A â†’ F B â†’ F A
  (fâ‚ >â‰¯ fâ‚‚) = fâ‚ >>= Î» result â†’ fâ‚‚ >> return result

  _>>=r_ : âˆ€{A B : Set â„“} â†’ F A â†’ (A â†’ B) â†’ F B
  a >>=r f = a >>= (return âˆ˜ f)

  _>>r_ : âˆ€{A B : Set â„“} â†’ F A â†’ B â†’ F B
  a >>r b = a >> return b
  
  _on-fail_>>=m_ : âˆ€ {A B : Set â„“} â†’ F (maybe A) â†’ F B â†’ (A â†’ F B) â†’ F B
  fa? on-fail fb >>=m fab = fa? >>= Î» {(just a) â†’ fab a; nothing â†’ fb}

  _on-fail_>>=s_ : âˆ€ {A B E : Set â„“} â†’ F (E âŠ A) â†’ (E â†’ F B) â†’ (A â†’ F B) â†’ F B
  fa+e on-fail feb >>=s fab = fa+e >>= Î» {(injâ‚ e) â†’ feb e; (injâ‚‚ a) â†’ fab a}
  
  return2 : âˆ€ {A B : Set â„“} â†’ A â†’ B â†’ F (A Ã— B)
  return2 a b = return (a , b)
  
  foldrM : âˆ€ {A B} â†’ (A â†’ F B â†’ F B) â†’ F B â†’ ğ•ƒ (F A) â†’ F B
  foldrM c n [] = n
  foldrM c n (fa :: fas) = fa >>= Î» a â†’ c a (foldrM c n fas)

  foldlM : âˆ€ {A B} â†’ (A â†’ F B â†’ F B) â†’ F B â†’ ğ•ƒ (F A) â†’ F B
  foldlM c n [] = n
  foldlM c n (fa :: fas) = fa >>= Î» a â†’ foldlM c (c a n) fas
  
  forM_init_use_ : âˆ€ {A B} â†’ ğ•ƒ (F A) â†’ F B â†’ (A â†’ F B â†’ F B) â†’ F B
  forM as init b use f = foldrM f b as
  
open monad â¦ƒ...â¦„ public

join : âˆ€ {â„“}{F : Set â„“ â†’ Set â„“}{A : Set â„“} â¦ƒ _ : monad F â¦„ â†’ F (F A) â†’ F A
join ffa = ffa >>= id

infixr 2 _>>âˆ˜_
_>>âˆ˜_ : âˆ€{â„“}{F : Set â„“ â†’ Set â„“}{A B : Set â„“} â¦ƒ _ : monad F â¦„ â†’ F A â†’ F (A â†’ F B) â†’ F B
a >>âˆ˜ f = a >>= Î» a â†’ f >>= Î» f â†’ f a


--========== Id ==========--
-- Using "id" itself causes Agda to hang when resolving instances, I suspect due
-- to something like endlessly embedding (id (id (id (...)))). So instead we must
-- use a "newtype" for id.

record Id (A : Set) : Set where
  constructor id-in
  field id-out : A
open Id public

instance
  id-functor : functor Id
  id-applicative : applicative Id
  id-monad : monad Id

  fmap â¦ƒ id-functor â¦„ f = id-in âˆ˜ (f âˆ˜ id-out)

  pure â¦ƒ id-applicative â¦„ = id-in
  _<*>_ â¦ƒ id-applicative â¦„ fab fa = id-in (id-out fab (id-out fa))

  return â¦ƒ id-monad â¦„ = id-in
  _>>=_ â¦ƒ id-monad â¦„ a f = f (id-out a)


--========== IO ==========--

instance
  IO-functor : functor IO
  IO-applicative : applicative IO
  IO-monad : monad IO

{-
postulate
  IO-functor-identity-law :
    âˆ€ {A} â†’
      fmap â¦ƒ IO-functor â¦„ {A} id â‰¡ id
  IO-functor-composition-law :
    âˆ€ {A B C} (f : B â†’ C) (g : A â†’ B) â†’
      fmap (f âˆ˜ g) â‰¡ fmap f âˆ˜ fmap g

  IO-applicative-identity-law :
    âˆ€ {A} (v : IO A) â†’
      pure â¦ƒ IO-applicative â¦„ id <*> v â‰¡ v
  IO-applicative-composition-law :
    âˆ€ {A B C} (u : IO (B â†’ C)) (v : IO (A â†’ B)) (w : IO A) â†’
      pure â¦ƒ IO-applicative â¦„ _âˆ˜_ <*> u <*> v <*> w â‰¡ u <*> (v <*> w)
  IO-applicative-homomorphism-law :
    âˆ€ {A B} (f : A â†’ B) (x : A) â†’
      pure â¦ƒ IO-applicative â¦„ f <*> pure x â‰¡ pure (f x)
  IO-applicative-interchange-law :
    âˆ€ {A B} (u : IO (A â†’ B)) (y : A) â†’
      u <*> pure y â‰¡ pure â¦ƒ IO-applicative â¦„ (_$ y) <*> u

  IO-monad-left-identity-law :
    âˆ€ {A B} (a : A) (k : A â†’ IO B) â†’
      (return a >>= k) â‰¡ k a
  IO-monad-right-identity-law :
    âˆ€ {A} (m : IO A) â†’
      (m >>= return) â‰¡ m
  IO-monad-associativity-law :
    âˆ€ {A B C} (m : IO A) (k : A â†’ IO B) (h : B â†’ IO C) â†’
      (m >>= (Î» x â†’ k x >>= h)) â‰¡ ((m >>= k) >>= h)
-}

  fmap â¦ƒ IO-functor â¦„ g fa = fa >>=áµ¢â‚’ Î» a â†’ returnáµ¢â‚’ (g a)

  pure â¦ƒ IO-applicative â¦„ = returnáµ¢â‚’
  _<*>_ â¦ƒ IO-applicative â¦„ fab fa = fab >>=áµ¢â‚’ Î» ab â†’ fa >>=áµ¢â‚’ Î» a â†’ returnáµ¢â‚’ (ab a)

  return â¦ƒ IO-monad â¦„ = returnáµ¢â‚’
  _>>=_ â¦ƒ IO-monad â¦„ = _>>=áµ¢â‚’_


--========== âŠ ==========--

instance
  sum-functor : âˆ€ {â„“ â„“'} {E : Set â„“} â†’ functor {â„“'} {â„“ âŠ” â„“'} (E âŠ_)
  sum-applicative : âˆ€ {â„“ â„“'} {E : Set â„“} â†’ applicative {â„“'} {â„“ âŠ” â„“'} (E âŠ_)
  sum-monad : âˆ€ {â„“ â„“'} {E : Set â„“} â†’ monad {â„“'} {â„“ âŠ” â„“'} (E âŠ_)

  fmap â¦ƒ sum-functor â¦„ f (injâ‚ e) = injâ‚ e
  fmap â¦ƒ sum-functor â¦„ f (injâ‚‚ a) = injâ‚‚ (f a)

  pure â¦ƒ sum-applicative â¦„ = injâ‚‚
  _<*>_ â¦ƒ sum-applicative â¦„ sf sa =
    sf >>= Î» f â†’
    sa >>= Î» a â†’
    return (f a)

  return â¦ƒ sum-monad â¦„ = injâ‚‚
  _>>=_ â¦ƒ sum-monad â¦„ (injâ‚ e) f = injâ‚ e
  _>>=_ â¦ƒ sum-monad â¦„ (injâ‚‚ a) f = f a


--========== maybe ==========--

instance
  maybe-functor : âˆ€ {â„“} â†’ functor {â„“} maybe
  maybe-applicative : âˆ€ {â„“} â†’ applicative {â„“} maybe
  maybe-monad : âˆ€ {â„“} â†’ monad {â„“} maybe
  
  fmap â¦ƒ maybe-functor â¦„ = maybe-map
  
  pure â¦ƒ maybe-applicative â¦„ = just
  _<*>_ â¦ƒ maybe-applicative â¦„ f? a? =
    f? â‰«=maybe Î» f â†’ a? â‰«=maybe (just âˆ˜ f)

  return â¦ƒ maybe-monad â¦„ = just
  _>>=_ â¦ƒ maybe-monad â¦„ = _â‰«=maybe_
  

--========== ğ•ƒ ==========--

instance
  list-functor : âˆ€ {â„“} â†’ functor {â„“} ğ•ƒ
  list-applicative : âˆ€ {â„“} â†’ applicative {â„“} ğ•ƒ
  list-monad : âˆ€ {â„“} â†’ monad {â„“} ğ•ƒ
  
  fmap â¦ƒ list-functor â¦„ = map
  
  pure â¦ƒ list-applicative â¦„ = [_]
  _<*>_ â¦ƒ list-applicative â¦„ fs as = map (Î» {(f , a) â†’ f a}) (zip fs as)

  return â¦ƒ list-monad â¦„ = [_]
  _>>=_ â¦ƒ list-monad â¦„ as f = concat (map f as)
